code/sha2-mb/Hacl.SHA2.Vec128.fst
@@ -10,7 +10,6 @@ open Lib.Buffer
 open Lib.MultiBuffer
 
 open Spec.Hash.Definitions
-open Hacl.Hash.Definitions
 open Hacl.Spec.SHA2.Vec
 open Hacl.Impl.SHA2.Generic
 
@@ -29,12 +28,13 @@ let sha224_update4 b hash = update #SHA2_224 #M128 b hash
 
 val sha224_4 (r0 r1 r2 r3: lbuffer uint8 28ul) (len:size_t) (b0 b1 b2 b3: lbuffer uint8 len) :
   Stack unit
-  (requires fun h0 -> live4 h0 b0 b1 b2 b3 /\ live4 h0 r0 r1 r2 r3 /\ internally_disjoint4 r0 r1 r2 r3)
+  (requires fun h0 -> v len <= max_input_length SHA2_224 /\
+    live4 h0 b0 b1 b2 b3 /\ live4 h0 r0 r1 r2 r3 /\ internally_disjoint4 r0 r1 r2 r3)
   (ensures  fun h0 _ h1 -> modifies (loc r0 |+| loc r1 |+| loc r2 |+| loc r3) h0 h1 /\
-    as_seq h1 r0 == Spec.hash #SHA2_224 (v len) (as_seq h0 b0) /\
-    as_seq h1 r1 == Spec.hash #SHA2_224 (v len) (as_seq h0 b1) /\
-    as_seq h1 r2 == Spec.hash #SHA2_224 (v len) (as_seq h0 b2) /\
-    as_seq h1 r3 == Spec.hash #SHA2_224 (v len) (as_seq h0 b3))
+    as_seq h1 r0 == Spec.hash SHA2_224 (as_seq h0 b0) /\
+    as_seq h1 r1 == Spec.hash SHA2_224 (as_seq h0 b1) /\
+    as_seq h1 r2 == Spec.hash SHA2_224 (as_seq h0 b2) /\
+    as_seq h1 r3 == Spec.hash SHA2_224 (as_seq h0 b3))
 
 let sha224_4 r0 r1 r2 r3 len b0 b1 b2 b3 =
   let h0 = ST.get() in
@@ -47,12 +47,11 @@ let sha224_4 r0 r1 r2 r3 len b0 b1 b2 b3 =
   loc_multi4 rb;
   hash #SHA2_224 #M128 sha224_update4 rb len ib;
   let h1 = ST.get() in
-  Hacl.Spec.SHA2.Equiv.hash_lemma #SHA2_224 #M128 (v len) (as_seq_multi h0 ib);
+  Hacl.Spec.SHA2.Equiv.hash_agile_lemma #SHA2_224 #M128 (v len) (as_seq_multi h0 ib);
   assert ((as_seq_multi h1 rb).(|0|) == as_seq h1 r0);
   assert ((as_seq_multi h1 rb).(|1|) == as_seq h1 r1);
   assert ((as_seq_multi h1 rb).(|2|) == as_seq h1 r2);
   assert ((as_seq_multi h1 rb).(|3|) == as_seq h1 r3)
-
 
 
 [@CInline]
