code/sha2-mb/Hacl.SHA2.Vec256.fst
@@ -10,14 +10,12 @@ open Lib.Buffer
 open Lib.MultiBuffer
 
 open Spec.Hash.Definitions
-open Hacl.Hash.Definitions
 open Hacl.Spec.SHA2.Vec
 open Hacl.Impl.SHA2.Generic
 
 module ST = FStar.HyperStack.ST
 module Spec = Spec.Agile.Hash
 module SpecVec = Hacl.Spec.SHA2.Vec
-
 
 #set-options "--z3rlimit 50 --fuel 0 --ifuel 0"
 
@@ -29,16 +27,17 @@ let sha224_update8 b hash = update #SHA2_224 #M256 b hash
 
 val sha224_8 (r0 r1 r2 r3 r4 r5 r6 r7 : lbuffer uint8 28ul) (len:size_t) (b0 b1 b2 b3 b4 b5 b6 b7 : lbuffer uint8 len) :
   Stack unit
-  (requires fun h0 -> live8 h0 b0 b1 b2 b3 b4 b5 b6 b7 /\ live8 h0 r0 r1 r2 r3 r4 r5 r6 r7 /\ internally_disjoint8 r0 r1 r2 r3 r4 r5 r6 r7)
-  (ensures  fun h0 _ h1 -> modifies (loc r0 |+| loc r1 |+| loc r2 |+| loc r3 |+| loc r4 |+| loc r5 |+| loc r6 |+| loc r7) h0 h1 /\
-    as_seq h1 r0 == Spec.hash #SHA2_224 (v len) (as_seq h0 b0) /\
-    as_seq h1 r1 == Spec.hash #SHA2_224 (v len) (as_seq h0 b1) /\
-    as_seq h1 r2 == Spec.hash #SHA2_224 (v len) (as_seq h0 b2) /\
-    as_seq h1 r3 == Spec.hash #SHA2_224 (v len) (as_seq h0 b3) /\
-    as_seq h1 r4 == Spec.hash #SHA2_224 (v len) (as_seq h0 b4) /\
-    as_seq h1 r5 == Spec.hash #SHA2_224 (v len) (as_seq h0 b5) /\
-    as_seq h1 r6 == Spec.hash #SHA2_224 (v len) (as_seq h0 b6) /\
-    as_seq h1 r7 == Spec.hash #SHA2_224 (v len) (as_seq h0 b7))
+  (requires fun h0 -> v len <= max_input_length SHA2_224 /\
+    live8 h0 b0 b1 b2 b3 b4 b5 b6 b7 /\ live8 h0 r0 r1 r2 r3 r4 r5 r6 r7 /\ internally_disjoint8 r0 r1 r2 r3 r4 r5 r6 r7)
+  (ensures  fun h0 _ h1 -> modifies (loc r0 |+| (loc r1 |+| (loc r2 |+| (loc r3 |+| (loc r4 |+| (loc r5 |+| (loc r6 |+| loc r7))))))) h0 h1 /\
+    as_seq h1 r0 == Spec.hash SHA2_224 (as_seq h0 b0) /\
+    as_seq h1 r1 == Spec.hash SHA2_224 (as_seq h0 b1) /\
+    as_seq h1 r2 == Spec.hash SHA2_224 (as_seq h0 b2) /\
+    as_seq h1 r3 == Spec.hash SHA2_224 (as_seq h0 b3) /\
+    as_seq h1 r4 == Spec.hash SHA2_224 (as_seq h0 b4) /\
+    as_seq h1 r5 == Spec.hash SHA2_224 (as_seq h0 b5) /\
+    as_seq h1 r6 == Spec.hash SHA2_224 (as_seq h0 b6) /\
+    as_seq h1 r7 == Spec.hash SHA2_224 (as_seq h0 b7))
 
 let sha224_8 r0 r1 r2 r3 r4 r5 r6 r7 len b0 b1 b2 b3 b4 b5 b6 b7 =
   let h0 = ST.get() in
@@ -51,7 +50,7 @@ let sha224_8 r0 r1 r2 r3 r4 r5 r6 r7 len b0 b1 b2 b3 b4 b5 b6 b7 =
   loc_multi8 rb;
   hash #SHA2_224 #M256 sha224_update8 rb len ib;
   let h1 = ST.get() in
-  Hacl.Spec.SHA2.Equiv.hash_lemma #SHA2_224 #M256 (v len) (as_seq_multi h0 ib);
+  Hacl.Spec.SHA2.Equiv.hash_agile_lemma #SHA2_224 #M256 (v len) (as_seq_multi h0 ib);
   assert ((as_seq_multi h1 rb).(|0|) == as_seq h1 r0);
   assert ((as_seq_multi h1 rb).(|1|) == as_seq h1 r1);
   assert ((as_seq_multi h1 rb).(|2|) == as_seq h1 r2);
@@ -113,12 +112,13 @@ let sha384_update4 b hash = update #SHA2_384 #M256 b hash
 
 val sha384_4 (r0 r1 r2 r3 : lbuffer uint8 48ul) (len:size_t) (b0 b1 b2 b3 : lbuffer uint8 len) :
   Stack unit
-  (requires fun h0 -> live4 h0 b0 b1 b2 b3 /\ live4 h0 r0 r1 r2 r3 /\ internally_disjoint4 r0 r1 r2 r3)
+  (requires fun h0 -> v len <= max_input_length SHA2_384 /\
+    live4 h0 b0 b1 b2 b3 /\ live4 h0 r0 r1 r2 r3 /\ internally_disjoint4 r0 r1 r2 r3)
   (ensures  fun h0 _ h1 -> modifies (loc r0 |+| loc r1 |+| loc r2 |+| loc r3) h0 h1 /\
-    as_seq h1 r0 == Spec.hash #SHA2_384 (v len) (as_seq h0 b0) /\
-    as_seq h1 r1 == Spec.hash #SHA2_384 (v len) (as_seq h0 b1) /\
-    as_seq h1 r2 == Spec.hash #SHA2_384 (v len) (as_seq h0 b2) /\
-    as_seq h1 r3 == Spec.hash #SHA2_384 (v len) (as_seq h0 b3))
+    as_seq h1 r0 == Spec.hash SHA2_384 (as_seq h0 b0) /\
+    as_seq h1 r1 == Spec.hash SHA2_384 (as_seq h0 b1) /\
+    as_seq h1 r2 == Spec.hash SHA2_384 (as_seq h0 b2) /\
+    as_seq h1 r3 == Spec.hash SHA2_384 (as_seq h0 b3))
 
 let sha384_4 r0 r1 r2 r3 len b0 b1 b2 b3 =
   let h0 = ST.get() in
@@ -131,7 +131,7 @@ let sha384_4 r0 r1 r2 r3 len b0 b1 b2 b3 =
   loc_multi4 rb;
   hash #SHA2_384 #M256 sha384_update4 rb len ib;
   let h1 = ST.get() in
-  Hacl.Spec.SHA2.Equiv.hash_lemma #SHA2_384 #M256 (v len) (as_seq_multi h0 ib);
+  Hacl.Spec.SHA2.Equiv.hash_agile_lemma #SHA2_384 #M256 (v len) (as_seq_multi h0 ib);
   assert ((as_seq_multi h1 rb).(|0|) == as_seq h1 r0);
   assert ((as_seq_multi h1 rb).(|1|) == as_seq h1 r1);
   assert ((as_seq_multi h1 rb).(|2|) == as_seq h1 r2);
